execution resources viewed as matrices viewed as functions

Execution_resources.v
@@ -1,6 +1,7 @@
 
 From Views Require Import utils.
 Require Import PeanoNat.
+From Views Require Import BoundedInt.
 
 (* Inductive execlevel: Type :=
   | Blocks
@@ -19,141 +20,138 @@ Inductive execexpr: Type :=
 Inductive exec_distrib: Type :=
   | Distrib (ed: exec_distrib) (distribs: list (execlevel * nat)). *)
 
+Inductive Thread_t : Type :=
+  | t (id : nat)
+.
+
+
+Definition shape : Type := nat * nat * nat.
+
+Definition Matrix (T : Type) (shp : shape) : Type :=
+  match shp with | (x,y,z) => Idx x -> Idx y -> Idx z -> T
+end.
+
+Definition Vector (T : Type) (n : nat) : Type :=
+  Idx n -> T
+.
+
+Definition Warp_t : Type := Vector Thread_t 32.
+Definition Block_t (shp : shape) : Type :=
+      match shp with | (x,y,z) => Matrix Thread_t (x, y, z) end.
+Definition Grid_t (shp : shape) (shp' : shape) : Type :=
+      match shp with | (x,y,z) => Matrix (Block_t shp') (x, y, z) end.
+
+Inductive execution_resource : Type :=
+  | thread (t : Thread_t)
+  | warp (w : Warp_t)
+  | block (shp : shape) (b : Block_t shp)
+  | grid (shp : shape) (shp' : shape) (g : Grid_t shp shp')
+  | Collection (n : nat) (content : Vector execution_resource n)
+  | Error
+.
+
+
+Definition build_block (shp : shape) (offset : nat) : Block_t shp :=
+  match shp with
+  | (x,y,z) => fun i j k => (t (offset + to_nat i + x*(to_nat j) + x*y*(to_nat k)))
+end.
+
+Definition build_grid (shp : shape) (shp' : shape) : Grid_t shp shp' :=
+  match shp with
+  | (x,y,z) => fun i j k => (build_block shp' (to_nat i + x*(to_nat j) + x*y*(to_nat k)))
+end.
+
+Definition build_warp : Warp_t :=
+  fun i => (t (to_nat i))
+.
+
+Definition Thread (id : nat) := thread (t id).
+Definition Warp := warp build_warp.
+Definition Block (shp : shape) := block shp (build_block shp 0).
+Definition Grid (shp : shape) (shp' : shape) := grid shp shp' (build_grid shp shp').
 
 Inductive dimension : Type :=
   | _x | _y | _z
 .
 
-Inductive shape : Type :=
-  | XYZ (x : nat) (y : nat) (z : nat)
-  | XY (x : nat) (y : nat)
-  | XZ (x : nat) (z : nat)
-  | YZ (y : nat) (z : nat)
-  | X (x : nat)
-  | Y (y : nat)
-  | Z (z : nat)
+
+Fixpoint for_all (e : execution_resource) (d : dimension) : execution_resource :=
+  match e,d with
+  | Collection n v,_ => Collection n (fun x => for_all (v x) d)
+  | grid (x,1,1) shp' g, _x => Collection x (fun i => block shp' (g i zero zero))
+  | grid (1,y,1) shp' g, _y => Collection y (fun j => block shp' (g zero j zero))
+  | grid (1,1,z) shp' g, _z => Collection z (fun k => block shp' (g zero zero k))
+  | grid (1,_,_) _ _, _x => Error
+  | grid (_,1,_) _ _, _y => Error
+  | grid (_,_,1) _ _, _z => Error
+  | grid (x,y,z) shp' g, _x => Collection x (fun i => grid (1,y,z) shp' (fun _ j k => g i j k))
+  | grid (x,y,z) shp' g, _y => Collection y (fun j => grid (x,1,z) shp' (fun i _ k => g i j k))
+  | grid (x,y,z) shp' g, _z => Collection z (fun k => grid (x,y,1) shp' (fun i j _ => g i j k))
+  | block (x,1,1) b, _x => Collection x (fun i => thread (b i zero zero))
+  | block (1,y,1) b, _y => Collection y (fun j => thread (b zero j zero))
+  | block (1,1,z) b, _z => Collection z (fun k => thread (b zero zero k))
+  | block (1,_,_) _, _x => Error
+  | block (_,1,_) _, _y => Error
+  | block (_,_,1) _, _z => Error
+  | block (x,y,z) b, _x => Collection x (fun i => block (1,y,z) (fun _ j k => b i j k))
+  | block (x,y,z) b, _y => Collection y (fun j => block (x,1,z) (fun i _ k => b i j k))
+  | block (x,y,z) b, _z => Collection z (fun k => block (x,y,1) (fun i j _ => b i j k))
+  | warp w, _x => Collection 32 (fun i => thread (w i))
+  | _,_ => Error
+end.
+
+Inductive Nested_List (T : Type) : Type :=
+  | Elt (x : T)
+  | Nest (l : List (Nested_List T))
 .
 
-Inductive execution_resource : Type :=
-  | Grid (s : shape) (s' : shape) (offset : nat) (step : nat*nat)
-  | Block (s : shape) (offset : nat) (step : nat*nat)
-  | Warp (offset : nat)
-  | Thread (id : nat)
-.
-
-Definition shapesize (s : shape) :=
-  match s with
-  | XYZ x y z => x*y*z
-  | XY x y => x*y
-  | XZ x z => x*z
-  | YZ y z => y*z
-  | X x => x
-  | Y y => y
-  | Z z => z
-end.
-
-Definition size (e : execution_resource) : nat :=
+Fixpoint to_list (e : execution_resource) : Nested_List execution_resource :=
   match e with
-  | Grid s s' _ _ => shapesize s * shapesize s'
-  | Block s _ _ => shapesize s
-  | Warp _ => 32
-  | Thread _ => 1
+  | Collection n v => Nest _ (rev (buildList (fun i => to_list (v i))))
+  | _ => Elt _ e
 end.
 
-Definition access_dimension (s : shape) (d : dimension) : option shape * nat :=
-  match s,d with
-  | XYZ x y z, _x => (Some (YZ y z), x)
-  | XYZ x y z, _y => (Some (XZ x z), y)
-  | XYZ x y z, _z => (Some (XY x y), z)
-  | XY x y, _x => (Some (Y y), x)
-  | XY x y, _y => (Some (X x), y)
-  | XZ x z, _x => (Some (Z z), x)
-  | XZ x z, _z => (Some (X x), z)
-  | YZ y z, _y => (Some (Z z), y)
-  | YZ y z, _z => (Some (Y y), z)
-  | X x, _x => (None, x)
-  | Y y, _y => (None, y)
-  | Z z, _z => (None, z)
-  | _,_ => (None,0)
+Notation "[ l ]" := (Nest _ l).
+Notation "# x" := (Elt _ x) (at level 20).
+
+Definition shiftBounded {a : nat} {b : nat} {n : nat} {i : Idx (b-a)} :
+  a + to_nat i < n.
+Proof.
+Admitted.
+
+Definition shift {n : nat} {b : nat} {a : nat} (i : Idx (b-a)) : Idx n :=
+  idx n (a + to_nat i) shiftBounded.
+
+Fixpoint select (e : execution_resource) (l : nat) (r : nat) (d : dimension) : execution_resource :=
+  match e,d with
+  | Collection n v,_ => Collection n (fun x => select (v x) l r d)
+  | grid (_,1,1) shp' g, _x => Collection (r-l) (fun i => block shp' (g (shift i) zero zero))
+  | grid (1,_,1) shp' g, _y => Collection (r-l) (fun j => block shp' (g zero (shift j) zero))
+  | grid (1,1,_) shp' g, _z => Collection (r-l) (fun k => block shp' (g zero zero (shift k)))
+  | grid (1,_,_) _ _, _x => Error
+  | grid (_,1,_) _ _, _y => Error
+  | grid (_,_,1) _ _, _z => Error
+  | grid (_,y,z) shp' g, _x => Collection (r-l) (fun i => grid (1,y,z) shp' (fun _ j k => g (shift i) j k))
+  | grid (x,_,z) shp' g, _y => Collection (r-l) (fun j => grid (x,1,z) shp' (fun i _ k => g i (shift j) k))
+  | grid (x,y,_) shp' g, _z => Collection (r-l) (fun k => grid (x,y,1) shp' (fun i j _ => g i j (shift k)))
+  | block (_,1,1) b, _x => Collection (r-l) (fun i => thread (b (shift i) zero zero))
+  | block (1,_,1) b, _y => Collection (r-l) (fun j => thread (b zero (shift j) zero))
+  | block (1,1,_) b, _z => Collection (r-l) (fun k => thread (b zero zero (shift k)))
+  | block (1,_,_) _, _x => Error
+  | block (_,1,_) _, _y => Error
+  | block (_,_,1) _, _z => Error
+  | block (_,y,z) b, _x => Collection (r-l) (fun i => block (1,y,z) (fun _ j k => b (shift i) j k))
+  | block (x,_,z) b, _y => Collection (r-l) (fun j => block (x,1,z) (fun i _ k => b i (shift j) k))
+  | block (x,y,_) b, _z => Collection (r-l) (fun k => block (x,y,1) (fun i j _ => b i j (shift k)))
+  | warp w, _x => Collection 32 (fun i => thread (w i))
+  | _,_ => Error
 end.
 
-Fixpoint decompose (l : nat) (e : execution_resource) (offset : nat) (size : nat) : List execution_resource :=
-  match l with
-  | 0 => []
-  | S l => match e with
-           | Grid s s' b step => Grid s s' (b+offset) step
-           | Block s b step => Block s (b+offset) step
-           | Warp b => Warp (b+offset)
-           | Thread id => Thread (id+offset)
-           end :: (decompose l e (offset+size) size)
-end.
-
-Definition get_x (s : shape) :=
-  match s with
-  | XYZ x _ _ | XY x _ | XZ x _ | X x => x
-  | _ => 1
-end.
-
-Definition get_y (s : shape) :=
-  match s with
-  | XYZ _ y _ | XY _ y | YZ y _ | Y y => y
-  | _ => 1
-end.
-
-Definition get_z (s : shape) :=
-  match s with
-  | XYZ _ _ z | XZ _ z | YZ _ z | Z z => z
-  | _ => 1
-end.
-
-
-Definition get_offset (e : execution_resource) (d : dimension) : nat :=
-  match e with
-  | Grid s s' b _ => match d with
-                   | _x => size (Block s' b (0,0))
-                   | _y => (get_x s) * size (Block s' b (0,0))
-                   | _z => (get_x s) * (get_y s) * size (Block s' b (0,0))
-                   end
-  | Block s b _ => match d with
-                 | _x => (get_x s) * size (Thread b)
-                 | _y => (get_y s) * size (Thread b)
-                 | _z => (get_z s) * size (Thread b)
-                 end
-  | Warp _ => 32
-  | Thread _ => 1
-end.
-
-Definition for_all (d : dimension) (e : execution_resource) : List (execution_resource) :=
-  match e with
-  | Grid s0 s' offset (sx,sz) => match (access_dimension s0 d),d with
-                        | (Some s, l),_x => decompose l (Grid s s' offset (sx,sz)) 0 (sx*(get_y s0))
-                        | (Some s, l),_y => decompose l (Grid s s' offset (sx*get_y s0,sz)) 0 sx
-                        | (Some s, l),_z => decompose l (Grid s s' offset (sx,sz/(get_x s0))) 0 sz
-                        | (None, l),_x => decompose l (Block s' (offset*shapesize s') (1,get_x s' * get_z s')) 0 (sx*shapesize s')
-                        | (None, l),_y => decompose l (Block s' (offset*shapesize s') (1,get_x s' * get_z s')) 0 (sx*shapesize s')
-                        | (None, l),_z => decompose l (Block s' (offset*shapesize s') (1,get_x s' * get_z s')) 0 (sz*shapesize s')
-                        end
-  | Block s0 offset (sx,sz) => match (access_dimension s0 d),d with
-                        | (Some s, l),_x => decompose l (Block s offset (sx,sz)) 0 (sx*(get_y s0))
-                        | (Some s, l),_y => decompose l (Block s offset (sx*get_y s0,sz)) 0 sx
-                        | (Some s, l),_z => decompose l (Block s offset (sx,sz/(get_x s0))) 0 sz
-                        | (None, l),_x => decompose l (Thread offset) 0 sx
-                        | (None, l),_y => decompose l (Thread offset) 0 sx
-                        | (None, l),_z => decompose l (Thread offset) 0 sz
-                        end
-  | Warp offset => decompose 32 (Thread offset) 0 1
-  | _ => []
-end.
-
-
-Definition grid (s : shape) (s' : shape) := Grid s s' 0 (1,get_x s * get_z s).
-Definition block (s : shape) := Block s 0 (1,get_x s * get_z s).
-Definition warp := Warp 0.
-Definition thread (id : nat) := Thread id.
-
-
-
-
+Example test :
+  to_list (for_all (for_all (select (Block (3,2,100)) 0 2 _z) _y) _x) = [ [] ].
+Proof.
+  simpl. unfold crop. simpl.
+  
 
 
 
